straight line code!

Judge.v
@@ -5,6 +5,7 @@ Require Import msl.msl_direct.
 Require Import Language.
 Require Import Types.
 Require Import List.
+Import ListNotations.
 Require Import ListSet.
 Require Import Subst.
  
@@ -12,6 +13,8 @@ Require Import Subst.
 Reserved Notation "P / G ⊢ s ::: O " (at level 0, no associativity).
 
 Definition ν := vv.
+
+Definition wf_subst θ := forall v, θ v = ν <-> v = ν.
 
 Inductive wf_type : type_env -> reft_type -> Prop :=
 | wf_reft_t : forall Γ b p, wf_prop Γ p ->
@@ -23,15 +26,19 @@ wf_prop : type_env -> reft_prop -> Prop :=
 | wf_tt : forall Γ, 
 (* ------------------------------------------------------------------- *)
             wf_prop Γ tt_r 
+
 | wf_rel : forall Γ e1 o e2, wf_expr Γ e1 -> wf_expr Γ e2 ->
 (* ------------------------------------------------------------------- *)
   wf_prop Γ (rel_r e1 o e2)
+
 | wf_not : forall Γ p, wf_prop Γ p -> 
 (* ------------------------------------------------------------------- *)
   wf_prop Γ (not_r p)
+
 | wf_and : forall Γ p1 p2, wf_prop Γ p1 -> wf_prop Γ p2 -> 
 (* ------------------------------------------------------------------- *)
   wf_prop Γ (and_r p1 p2)
+
 | wf_or : forall Γ p1 p2, wf_prop Γ p1 -> wf_prop Γ p2 -> 
 (* ------------------------------------------------------------------- *)
   wf_prop Γ (or_r p1 p2)
@@ -41,12 +48,20 @@ wf_expr : type_env -> expr -> Prop :=
 | wf_val : forall Γ v,
 (* ------------------------------------------------------------------- *)
   wf_expr Γ (value_e v)
+
 | wf_var : forall Γ v t, (v,t) ∈ Γ ->
 (* ------------------------------------------------------------------- *)
   wf_expr Γ (var_e v)
+
 | wf_vv : forall Γ,
 (* ------------------------------------------------------------------- *)
-  wf_expr Γ (var_e ν).
+  wf_expr Γ (var_e ν)
+
+| wf_op : forall Γ f e1 e2,
+            wf_expr Γ e1 -> wf_expr Γ e2 ->
+(* ------------------------------------------------------------------- *)
+  wf_expr Γ (fun_e f e1 e2).
+            
 
 (* Definition wf_env Γ :=  *)
 (*   var_not_in ν Γ /\ Forall (fun xt => wf_type Γ (snd xt)) Γ. *)
@@ -57,47 +72,65 @@ Inductive wf_env : type_env -> Prop :=
     wf_env nil
   | wf_env_var : 
       forall Γ x T, 
-        wf_env Γ -> (x <> ν) -> var_not_in x Γ -> wf_type Γ T ->
+        wf_env Γ -> (x <> ν) -> var_not_in x Γ -> wf_type ((x,T) :: Γ) T ->
 (* ------------------------------------------------------------------- *)
     wf_env ((x, T) :: Γ).
 
-Inductive wf_schema : type_env -> proc_schema -> Prop :=
+Inductive wf_schema : proc_schema -> Prop :=
 | wf_proc_schema : 
-    forall Γ S, 
-      NoDup (proc_formals S) -> 
-      Forall (fun x => ~ (var_in x Γ)) (proc_formals S) ->
-      ~ (var_in (fst (proc_ret S)) Γ) ->
-      Forall (wf_type (ext_type_env Γ (proc_args S))) (proc_formal_ts S) ->
-      wf_type (ext_type_env Γ (proc_args S)) (snd (proc_ret S)) ->
+    forall S, 
+      length (s_formals S) = length (s_formal_ts S) ->
+      wf_env (combine (s_formals S) (s_formal_ts S)) ->
+      (* Forall (wf_type (ext_type_env Γ (proc_args S))) (proc_formal_ts S) -> *)
+      wf_env (s_ret S :: (combine (s_formals S) (s_formal_ts S))) ->
 (* ------------------------------------------------------------------- *)
-  wf_schema Γ S.
+  wf_schema S.
 
 Inductive expr_type : type_env -> expr -> reft_type -> Prop :=
 | t_const : forall Γ v,
 (* ------------------------------------------------------------------- *)
   expr_type Γ (value_e v) { ν : (base_of_val v) | (var_e ν) .= (value_e v) }
-
+            
 | t_var : forall Γ x τ φ, (x, { ν : τ | φ }) ∈ Γ ->
 (* ------------------------------------------------------------------- *)
   expr_type Γ (var_e x) { ν : τ | φ }.
 
-Definition tc_list Γ (xs : list var) (ts : list reft_type) :=
-  Forall (fun xt => expr_type Γ (var_e (fst xt)) (snd xt))
-         (combine xs ts).
+Definition tc_list Γ (xts : list (var * reft_type)) :=
+  Forall (fun xt => 
+            expr_type Γ (var_e (fst xt)) (snd xt)) xts.
 
-Definition subst_call S (xs : list var) := combine (proc_formals S) xs.
+Fixpoint subst_of_list (sub : list (var*var)) : subst_t var var :=
+  fun i => 
+    match sub with
+      | (x,x') :: sub' => if eq_dec i x then x' else subst_of_list sub' i
+      | _ => i
+    end.
+
+Definition subst_call S (xr : var) (xs : list var) := 
+  subst_of_list ((fst (s_ret S), xr) :: (combine (s_formals S) xs)).
                               
 Inductive stmt_type : proc_env -> type_env -> stmt -> type_env -> Prop :=
 | t_skip : forall Φ Γ,
 (* ------------------------------------------------------------------- *)
   (Φ / Γ ⊢ skip_s ::: Γ)
 | t_proc_s : 
-    forall Φ Γ (v:var) p S xs θ,
-      (p,S) ∈ Φ -> wf_schema nil S -> (θ = subst_call S xs) ->
-      var_not_in v Γ -> v <> ν ->
-      tc_list Γ xs (subst θ (proc_formal_ts S)) ->
+    forall Φ Γ (v:var) f p S xs ts θ θS,
+      (f,(p,S)) ∈ Φ -> 
+      wf_schema S -> 
+      (* (θ = subst_call S v xs) -> *)
+      wf_subst θ ->
+      θS = subst θ S ->
+      xs = subst θ (s_formals S) ->
+      ts = subst θ (s_formal_ts S) ->
+      v  = subst θ (fst (s_ret S)) ->
+      (forall x, θ x = v <-> x = (fst (s_ret S))) ->
+      (forall x', ~(In x' (fst (s_ret S) :: s_formals S)) -> θ x' = x') ->
+      (* v <> ν -> var_not_in v Γ ->  *)
+      wf_env (subst θ (s_ret S) :: Γ) ->
+      Forall (fun t => wf_type Γ t) ts ->
+      tc_list Γ (combine xs ts) ->
 (* ------------------------------------------------------------------- *)
-  (Φ / Γ ⊢ proc_s v p xs ::: ((v, subst θ (snd (proc_ret S))) :: Γ))
+  (Φ / Γ ⊢ proc_s f xs [v] ::: (subst θ (s_ret S) :: Γ))
 | t_assign : 
     forall Φ Γ v e τ φ, v <> ν ->
       var_not_in v Γ -> expr_type Γ e { ν : τ | φ } ->
@@ -107,6 +140,7 @@ Inductive stmt_type : proc_env -> type_env -> stmt -> type_env -> Prop :=
   (Φ / Γ ⊢ s1 ::: Γ') -> (Φ / Γ' ⊢ s2 ::: Γ'') ->
 (* ------------------------------------------------------------------- *)
   (Φ / Γ ⊢ seq_s s1 s2 ::: Γ'')
+
 where "P / G ⊢ s ::: O " := (stmt_type P G s O).
 
 
