ProgramLogic.v
@@ -1,16 +1,15 @@
 Add LoadPath "vst".
+
+Require Import Subst.
 Require Import Language.
 Require Import msl.msl_direct.
 
 Delimit Scope logic_scope with logic.
 
-Definition world := var -> option value.
-Definition den (s: state) : world := table_get s.
-Definition defined (y: var) : pred world :=
-   fun w => exists v, w y = Some v.
+Definition world := state.
 
 Definition eval_to (e: expr) (v:value) : pred world :=
-  fun w => eval w e = Some v.
+  fun w => eval w e = v.
 
 Instance Join_world: Join world := Join_equiv world.
 
@@ -22,56 +21,75 @@ Instance Disj_world : Disj_alg world := _.
 Definition fun_set (f: var -> option value) (x: var) (y: option value) :=
   fun i => if eq_dec i x then y else f i.
 
-Definition subst_one (x : var) (v : expr) :=
-  fun i => if eq_dec i x then Some v else None.
+Definition subst_one (x : var) (e : expr) :=
+  fun i => if eq_dec i x then e else (var_e i).
 
 Definition subst_pred sub (P: pred world) : (pred world) := 
   fun w =>
-    P (fun i => match sub i with
-                  | None    => w i
-                  | Some e  => eval w e
-                end).
+    P (fun i => eval w (sub i)).
+
+Definition subst_pred_var sub (P: pred world) : pred world :=
+  fun w =>
+    P (fun i => eval w (var_e (sub i))).
+    
+Instance Subst_pred_var : Subst (pred world) var var := subst_pred_var.
+Instance Subst_pred : Subst (pred world) var expr := subst_pred.
                  
 Definition equal (x y: var) : pred world :=
   fun w => w x = w y.
 
 Inductive modvars : stmt -> var -> Prop :=
 | mod_assign: forall x e, modvars (assign_s x e) x
+| mod_proc: forall x f xs os, 
+              In x os ->
+              modvars (proc_s f xs os) x
 | mod_seq1: forall x s1 s2, modvars s1 x -> modvars (seq_s s1 s2) x
 | mod_seq2: forall x s1 s2, modvars s2 x -> modvars (seq_s s1 s2) x.
 
 Definition nonfreevars (P: pred world) (x: var) : Prop :=
-  forall stk v, P stk -> P (fun_set stk x v).
+  forall stk v, P stk -> subst_pred (subst_one x v) P stk.
 
 Definition subset (S1 S2 : var -> Prop) := forall x, S1 x -> S2 x.
 
-(* Inductive safe : (list stmt * state) -> Prop := *)
-(* | safe_step: forall s1 s2, step s1 s2 -> safe s2 -> safe s1 *)
-(* | safe_halt: forall s, safe (nil, s). *)
+Definition procspec := (pname * proc * pred world * pred world)%type.
+  
+Definition procspecs := list procspec.
 
-(* Definition guards (P: pred world) (ss : list stmt) : Prop := *)
-(*   forall s, P (den s) -> safe (ss, s). *)
+Definition not_free_in (v : var) (v' : var) := v <> v'.
 
-Inductive semax : pred world -> stmt -> pred world -> Prop :=
+Definition unique_sub s (v : var) :=
+  exists v', (s v = v' /\ (forall x, x <> v -> not_free_in v' (s x))).
+
+Inductive semax : procspecs -> pred world -> stmt -> pred world -> Prop :=
   | semax_skip : 
-      forall P, semax P skip_s P
+      forall F P, semax F P skip_s P
   | semax_assign :
-      forall P x e,
-        semax (EX v : value, 
+      forall F P x e,
+        semax F (EX v : value, 
                       eval_to e v 
                    && subst_pred (subst_one x e) P) (assign_s x e)  P 
-  (* | semax_proc : *)
-  (*     forall  *)
+  | semax_proc :
+      forall f p (F : procspecs) P Q,
+        In (f, p, P, Q) F ->
+        semax F P (proc_s f (p_args stmt p) (p_mod stmt p)) Q
   | semax_seq : 
-      forall P Q R s1 s2,
-        semax P s1 Q -> semax Q s2 R -> 
-        semax P (seq_s s1 s2) R
+      forall F P Q R s1 s2,
+        semax F P s1 Q -> semax F Q s2 R -> 
+        semax F P (seq_s s1 s2) R
+  | semax_subst :
+      forall F P s Q θ,
+        semax F P s Q -> (forall x, (modvars s x -> unique_sub θ x)) ->
+        semax F (subst θ P) (subst θ s) (subst θ Q)
   | semax_pre_post :
-      forall P P' s Q Q',
-        (P |-- P') -> (Q' |-- Q) -> semax P' s Q' ->
-        semax P s Q.
-  
-Notation "{{ P }} s {{ Q }}" := (semax P%pred s Q%pred) (at level 90).
+      forall F P P' s Q Q',
+        (P |-- P') -> (Q' |-- Q) -> semax F P' s Q' ->
+        semax F P s Q
+  | semax_frame :
+      forall F P Q R s,
+        semax F P s Q -> subset (modvars s) (nonfreevars R) ->
+        semax F (P * R)%pred s (Q * R)%pred.
+
+Notation "F |- {{ P }} s {{ Q }}" := (semax F P%pred s Q%pred) (no associativity, at level 90).
 
 (* Definition x:var := 0. *)
 
