Subst.v
@@ -3,33 +3,31 @@ Add LoadPath "vst".
 Require Import Coq.Unicode.Utf8.
 Require Import msl.eq_dec.
 Require Import List.
+Import ListNotations.
 
-Definition subst_t (X : Type) := list (X * X).
+Definition subst_t (D : Type) (R : Type) := D -> R.
 
 (* Definition wf_subst{A : Type} (s : subst_t A) : Prop  := NoDup (fst (split s)). *)
 
-Class Subst (A X : Type) : Type :=
-  subst: subst_t X -> A -> A.
+Class Subst (A D R : Type) : Type :=
+  subst: subst_t D R -> A -> A.
 
-Fixpoint subst_prod (A X : Type) (SX : Subst X X) (s : subst_t X) (p : (X * A)) :=
+Fixpoint subst_prod (A B D R : Type) (SA : Subst A D R) (SB : Subst B D R) (s : subst_t D R) (p : (A * B)) :=
   match p with
-    | (p1, p2) => (subst s p1, p2)
+    | (p1, p2) => (subst s p1, subst s p2)
   end.
 
-Instance Subst_prod (A X : Type) (SX : Subst X X) : Subst (X * A) X := subst_prod A X SX.
+Instance Subst_prod (A B D R : Type) (SA : Subst A D R) (SB : Subst B D R): Subst (A * B) D R := 
+  subst_prod A B D R SA SB.
 
-Fixpoint subst_list (A X : Type) (SAX : Subst A X) (s : subst_t X) (l : list A) :=
+Fixpoint subst_list (A D R : Type) (SA : Subst A D R) (s : subst_t D R) (l : list A) :=
   match l with
-    | nil => nil
-    | h :: t => subst s h :: subst_list A X SAX s t
+    | nil => []
+    | h :: t => subst s h :: subst_list A D R SA s t
   end.
   
-Instance Subst_list (A X : Type) (SAX : Subst A X) : Subst (list A) X := subst_list A X SAX.
-
-Instance Subst_prod_list (A X : Type) (S : Subst X X) : Subst (list (X * A)) X := 
-  subst_list (X * A) X (Subst_prod A X S).
-
-Definition wf_subst (X : Type) (s : subst_t X) :=
-  NoDup (fst (split s)).
-
-(* Notation "[ e / x ]" := subst ((x, e) :: nil). *)
+Instance Subst_list (A D R : Type) (SA : Subst A D R) : Subst (list A) D R := 
+  subst_list A D R SA.
+(* Instance Subst_prod_list (A B D R : Type) (S : Subst A D R) : Subst (list (A * A)) D R := _. *)
+(* Definition wf_subst (X : Type) (s : subst_t X) := *)
+(*   NoDup (fst (split s)). *)
