Translation.v
@@ -6,6 +6,7 @@ Require Import Language.
 Require Import Judge.
 Require Import Subst.
 Require Import List.
+Import ListNotations.
 Require Import msl.msl_direct.
 Require Import Coq.Unicode.Utf8.
 
@@ -21,23 +22,14 @@ Open Scope pred.
 
 (** The meat of the sauce :d tasty **)
 Definition sep_base (x:var) (t:base_type) : pred world :=
-  EX v : (base_of_type t), (fun s => (eval s (var_e x) = Some (val_of_base t v))).
+  EX v : (base_of_type t), (fun s => (eval s (var_e x) = (val_of_base t v))).
 
 Fixpoint sep_pred (p:reft_prop) : pred world :=
   match p with
     | tt_r  => TT
     | rel_r e1 o e2 =>
       match o with
-        | eq_brel => 
-          EX v1 : value, EX v2 : value, 
-             !! (v1 = v2) 
-          && (fun s => Some v1 = (eval s e1)) 
-          && (fun s => Some v2 = (eval s e2))
-        | lt_brel => 
-          EX v1 : nat, EX v2 : nat, 
-             !! (v1 < v2) 
-          && (fun s => Some (int_v v1) = (eval s e1)) 
-          && (fun s => Some (int_v v2) = (eval s e2))
+        | eq_brel => (fun s => eval s e1 = eval s e2)
       end
     | not_r p => (sep_pred p) --> FF
     | and_r p1 p2 => sep_pred p1 && sep_pred p2
@@ -51,11 +43,28 @@ Definition sep_ty (x:var) (t:reft_type) : pred world :=
                                        && (sep_pred p))
   end.
 
+Definition sep_ty' (x:var) (t:reft_type) : pred world :=
+  match t with
+  | mkReft_type v b p => sep_base x b && (sep_pred (subst (subst_one v (var_e x)) p))
+  end.
+
 Fixpoint sep_env (Γ : type_env) : pred world :=
   match Γ with
     | nil => TT
     | (x,t) :: Γ' => sep_ty x t && sep_env Γ'
   end.
 
-Definition disj_subst Γ (θ : var -> option expr) :=
-  θ ν = None /\ forall x, var_in x Γ -> θ x = None.
+Definition sep_schema (f:pname) (s:stmt) (S:proc_schema) : procspec := 
+  match S with
+    | mkSchema xs ts (x, t) =>
+      (f, mkProc (length xs) xs [x] s, sep_env (combine xs ts), sep_ty x t)
+  end.
+
+Fixpoint sep_proc_env (Φ : proc_env) : procspecs :=
+  match Φ with
+    | nil => nil
+    | (f,(s,t)) :: Φ' => sep_schema f s t :: sep_proc_env Φ'
+  end.
+
+Definition disj_subst Γ (θ : var -> expr) :=
+  θ ν = (var_e ν) /\ forall x, var_in x Γ -> θ x = (var_e x).
