Types.v
@@ -12,31 +12,26 @@ Delimit Scope reft_scope with reft.
 
 (** Type Language **)
 Inductive base_type : Set :=
-  | int_t  : base_type
-  | bool_t : base_type.
+  | int_t  : base_type.
 
 Definition base_of_type b :=
   match b with
     | int_t => nat
-    | bool_t => bool
   end.
 
 Definition base_of_val (v: value) :=
   match v with
     | int_v  _ => int_t
-    | bool_v _ => bool_t
   end.
 
 Definition val_of_base : forall (b : base_type), (base_of_type b) -> value :=
   fun b => 
     match b with
       | int_t => fun x => int_v x
-      | bool_t => fun x => bool_v x
     end.
 
 Inductive brel : Set :=
-  | eq_brel : brel
-  | lt_brel : brel.
+  | eq_brel : brel.
 
 Inductive reft_prop : Set :=
   | tt_r   : reft_prop
@@ -50,7 +45,16 @@ Record reft_type : Set :=
                 reft_base: base_type;
                 reft_r: reft_prop } .
 
-Fixpoint subst_prop (s : subst_t var) prop :=
+Fixpoint subst_prop_var (s : subst_t var var) prop :=
+  match prop with
+    | tt_r          => tt_r
+    | rel_r e1 o e2 => rel_r (subst s e1) o (subst s e2)
+    | not_r p       => not_r (subst_prop_var s p)
+    | and_r p1 p2   => and_r (subst_prop_var s p1) (subst_prop_var s p2)
+    | or_r p1 p2    => or_r (subst_prop_var s p1) (subst_prop_var s p2)
+  end.
+
+Fixpoint subst_prop (s : subst_t var expr) prop :=
   match prop with
     | tt_r          => tt_r
     | rel_r e1 o e2 => rel_r (subst s e1) o (subst s e2)
@@ -59,28 +63,38 @@ Fixpoint subst_prop (s : subst_t var) prop :=
     | or_r p1 p2    => or_r (subst_prop s p1) (subst_prop s p2)
   end.
 
-Instance Subst_prop : Subst reft_prop var := subst_prop.
+Instance Subst_prop_var : Subst reft_prop var var := subst_prop_var.
+Instance Subst_prop : Subst reft_prop var expr := subst_prop.
+
+Definition subst_r_var (s : subst_t var var) reft :=
+  mkReft_type (subst s (reft_vv reft))
+              (reft_base reft)
+              (subst s (reft_r reft)).
 
 Definition subst_r s reft :=
   mkReft_type (reft_vv reft)
               (reft_base reft)
               (subst s (reft_r reft)).
 
-Instance Subst_reft : Subst reft_type var := subst_r.
+Instance Subst_reft_var : Subst reft_type var var := subst_r_var.
+Instance Subst_reft : Subst reft_type var expr := subst_r.
 
 Definition type_binding : Set := (var * reft_type)%type.
 
 Record proc_schema : Set :=
-  mkSchema { proc_args: list type_binding;
-              proc_ret: type_binding }.
+  mkSchema { s_formals: list var;
+             s_formal_ts: list reft_type;
+             s_ret: type_binding }.
 
-Definition proc_formals s := fst (List.split (proc_args s)).
-Definition proc_formal_ts s := snd (List.split (proc_args s)).
-
-Definition proc_binding : Set := (pname * proc_schema)%type.
+Definition subst_schema s S :=
+  let subst_both s xt := (subst s (fst xt), subst s (snd xt)) in
+  match S with
+    | mkSchema xs ts xt =>
+      mkSchema (subst s xs) (subst s ts) (subst_both s xt)
+  end.
+Instance Subst_proc_schema : Subst proc_schema var var := subst_schema.
 
 Notation "x .= y" := (rel_r x eq_brel y) (at level 70).
-Notation "x .< y" := (rel_r x lt_brel y) (at level 70).
 Notation "{ v : t | P }" := (mkReft_type v t P%reft) (at level 0, v at level 99, no associativity).
 
 
@@ -88,7 +102,7 @@ Notation "{ v : t | P }" := (mkReft_type v t P%reft) (at level 0, v at level 99,
 
 Definition bind_env (B T : Type) := list (B * T)%type.
 Definition type_env : Type := bind_env var reft_type.
-Definition proc_env : Type := bind_env pname proc_schema.
+Definition proc_env : Type := bind_env pname (stmt * proc_schema)%type.
 
 Definition var_in : var -> type_env -> Prop := 
   fun x Γ => exists t, In (x, t) Γ.
@@ -96,7 +110,7 @@ Definition var_in : var -> type_env -> Prop :=
 Definition var_not_in : var -> type_env -> Prop :=
   fun x Γ => Forall (fun xt => (fst xt <> x)) Γ.
 
-Definition fun_in : (pname * proc_schema) -> proc_env -> Prop :=
+Definition fun_in : (pname * (stmt * proc_schema)) -> proc_env -> Prop :=
   fun ft Φ => In ft Φ.
 
 Notation "X ∈ Y" := (In X Y) (at level 40).
