EvalLemmas.v
@@ -13,38 +13,46 @@ Require Import Tactics.
 
 Open Scope pred.
 
-Lemma var_val : 
-  forall Γ x b φ w,  (x,{ ν : b | φ}) ∈ Γ -> 
-                       sep_env Γ w -> 
-                       (EX v : (base_of_type b), 
-                               (fun s => eval s (var_e x) = Some (val_of_base b v))) w.
+Lemma var_val :
+  forall Γ x b φ w,  (x,{ ν : b | φ}) ∈ Γ ->
+                       sep_env Γ w ->
+                       (EX v : (base_of_type b),
+                               (fun s => eval s (var_e x) = val_of_base b v)) w.
 Proof.
-  induction Γ. crush_sep False fail.  
+  induction Γ. 
+  crush_sep False fail.
   crush_sep False fail.
   fold (subst_pred (subst_one ν (var_e x)) (sep_base ν b0) w) in H.
-  rewrite subst_vv_base_ap in H.
-  apply H.
-  crush_sep False fail.
+  unfold subst_one in H.
+  unfold subst_pred in H.
+  unfold sep_base in H.
+  destruct H.
+  destruct b0.
+  simpl in *.
+  exists x0.
+  foo.
+  specialize (IHΓ x b0 φ w).
+  destruct b0. simpl in *.
+  apply IHΓ; assumption.
 Qed.
 
 Lemma var_eval :
-  forall Γ x b φ w, (x, { ν : b | φ }) ∈ Γ -> sep_env Γ w -> (EX v : value, (fun s => eval s (var_e x) = Some v)) w.
+  forall Γ x b φ w, (x, { ν : b | φ }) ∈ Γ -> sep_env Γ w -> (EX v : value, (fun s => eval s (var_e x) = v)) w.
 Proof.
   crush_sep False fail.
   apply var_val with (x := x) (b := b) (φ := φ)in H0 .
   destruct H0.
   destruct b. simpl in *. exists (int_v x0). assumption.
-              simpl in *. exists (bool_v x0). assumption.
-  assumption. 
+  assumption.
 Qed.
 
-Lemma expr_eval : 
-  forall Γ e b φ w, 
+Lemma expr_eval :
+  forall Γ e b φ w,
     sep_env Γ w -> expr_type Γ e { ν : b | φ } ->
-                (EX v : value, (fun s => eval s e = Some v)) w.
+                (EX v : value, (fun s => eval s e = v)) w.
 Proof.
-  autounfold in *. intros. 
-  inversion H0. 
+  autounfold in *. intros.
+  inversion H0.
   subst.
   simpl. exists v. reflexivity.
   subst.
@@ -52,35 +60,31 @@ Proof.
 Qed.
 
 Lemma expr_eval_ty :
-  forall Γ e b φ w, 
-    sep_env Γ w -> expr_type Γ e { ν : b | φ } -> 
-      (EX v : base_of_type b , (fun s => eval s e = Some (val_of_base b v))) w.
+  forall Γ e b φ w,
+    sep_env Γ w -> expr_type Γ e { ν : b | φ } ->
+      (EX v : base_of_type b , (fun s => eval s e = val_of_base b v)) w.
 Proof.
   autounfold in *. intros.
-  destruct e. 
+  destruct e.
   + destruct b.
-  - inversion H0. subst.
-    destruct v. 
-    * simpl. exists n. reflexivity.
-    * simpl. exists b. reflexivity.
   - inversion H0. subst.
     destruct v.
     * simpl. exists n. reflexivity.
-    * simpl. exists b. reflexivity.
   + inversion H0. subst.
     * simpl. pose (var_val Γ v b φ w H4 H). assumption.
+  + inversion H0.
 Qed.
 
-Lemma expr_eval_derives :
-  forall Γ e b φ, 
-    expr_type Γ e { ν : b | φ } -> (sep_env Γ) |-- (EX v : value, (fun s => eval s e = Some v)).
-Proof.
-  intros Γ e b φ T w Den_Γ.
-  destruct e.
-  exists v. reflexivity.
-  apply var_eval with (x := v) (b := b) (φ := φ) in Den_Γ .
-  auto. inversion T. apply H2.
-Qed.
+(* Lemma expr_eval_derives : *)
+(*   forall Γ e b φ,  *)
+(*     expr_type Γ e { ν : b | φ } -> (sep_env Γ) |-- (EX v : value, (fun s => eval s e = Some v)). *)
+(* Proof. *)
+(*   intros Γ e b φ T w Den_Γ. *)
+(*   destruct e. *)
+(*   exists v. reflexivity. *)
+(*   apply var_eval with (x := v) (b := b) (φ := φ) in Den_Γ . *)
+(*   auto. inversion T. apply H2. *)
+(* Qed. *)
 
 Lemma subst_env_eq_expr:
   forall G b x e w φ, 
@@ -92,65 +96,45 @@ Proof.
   intros G b x e w φ etype senv H.
   pose (expr_eval_ty G e b φ w senv etype) as H0.
   rewrite subst_env_cons.
-  split.
-  unfold subst_pred.
-  unfold subst_one.
-  unfold sep_ty.
-  split.
-  unfold sep_base.
-  unfold subst_one. 
-  destruct H0.
-  exists x0.
-  simpl.
-  destruct (eq_dec ν ν).
-  simpl.
-  destruct (eq_dec x x). assumption. contradiction n; reflexivity. contradiction n; reflexivity.
-
-  unfold sep_pred.
-  destruct H0.
-  destruct b.
-  simpl in x0.
-  simpl in H0.
-  exists (int_v x0).
-  exists (int_v x0).
-  constructor. constructor. constructor.
-  simpl. unfold subst_one. simpl.
-  destruct (eq_dec ν ν).
-  simpl.
-  destruct (eq_dec x x).
-  symmetry.
-  assumption.
-  intuition.
-  intuition.
-  unfold subst_one.
-  destruct e. 
-  simpl. symmetry. apply H0.
-  simpl. inversion etype. subst. simpl. 
-  destruct (eq_dec v ν). simpl. 
-  destruct (eq_dec x x). simpl. 
-  symmetry. apply H0.
-  intuition.
-  intuition.
-  destruct (eq_dec v x). symmetry. apply H0. symmetry. apply H0.
-  
-  simpl in *.
-  symmetry in H0.
-  exists (bool_v x0).
-  exists (bool_v x0).
-  repeat constructor.
-  unfold subst_one. 
-  destruct (eq_dec ν ν).
-  simpl.
-  destruct (eq_dec x x).
-  simpl.
-  apply H0. intuition. intuition.
-  destruct e.
-  apply H0.
-  simpl. inversion etype. subst. 
-  unfold subst_one.
-  destruct (eq_dec v ν). simpl.
-  destruct (eq_dec x x). 
-  apply H0. intuition.
-  destruct (eq_dec v x). apply H0. apply H0.
-  assumption.
+  split. {
+    split. {
+      unfold subst_pred.
+      unfold subst_one.
+      unfold sep_ty.
+      unfold sep_base.
+      unfold subst_one. 
+      destruct H0.
+      exists x0.
+      simpl.
+      destruct (eq_dec ν ν).
+      + simpl.
+        destruct (eq_dec x x). 
+        * assumption. 
+        * contradiction n; reflexivity. 
+      + contradiction n; reflexivity.
+    } 
+    {
+      unfold sep_pred.
+      simpl.
+      unfold subst_one.
+      simpl.
+      destruct (eq_dec ν ν).
+      simpl. 
+      destruct e.
+      destruct (eq_dec x x).
+      simpl.
+      reflexivity.
+      contradiction n. reflexivity.
+      destruct (eq_dec x x). simpl.
+      destruct (eq_dec v ν). simpl.
+      destruct (eq_dec x x). reflexivity.
+      contradiction n.
+      simpl. destruct (eq_dec v x). reflexivity. reflexivity. contradiction n. reflexivity.
+      inversion etype.
+      contradiction n. reflexivity.
+    } 
+  }
+  {
+    assumption.
+  }
 Qed.
