TranslationLemmas.v
@@ -4,6 +4,7 @@ Require Import Coq.Unicode.Utf8.
 
 Require Import Types.
 Require Import Judge.
+Require Import Subst.
 Require Import ProgramLogic.
 Require Import Translation.
 Require Import Language.
@@ -11,6 +12,26 @@ Require Import WFLemmas.
 Require Import SubstLemmas.
 Require Import EvalLemmas.
 Require Import Tactics.
+Require Import List.
+Import ListNotations.
+
+Lemma forall_p_combine :
+  forall (X Y : Type) (P : Y -> Prop) (xs : list X) (ys : list Y),
+    length xs = length ys ->
+    Forall P ys -> 
+    Forall (fun xy => P (snd xy)) (combine xs ys).
+Proof.
+  intros.
+  rewrite Forall_forall in *.
+  intros.
+  destruct x as [x y].
+  simpl in *.
+  pose (combine_split xs ys H).
+  specialize (H0 y).
+  apply in_combine_r in H1.
+  apply H0.
+  assumption.
+Qed.
 
 Lemma type_interp :
   forall Γ x T s,
@@ -50,18 +71,56 @@ Proof.
         }
 Qed.
 
+Lemma types_interp :
+  forall Γ xs ts s,
+    sep_env Γ s ->
+    tc_list Γ (combine xs ts) ->
+    sep_env (combine xs ts) s.
+Proof.
+  intros.
+  unfold tc_list in H0.
+  rewrite Forall_forall in H0.
+  unfold sep_env.
+  induction (combine xs ts).
+  + constructor.
+  + destruct a. split.
+    apply type_interp with (Γ := Γ).
+    assumption. apply H0 with (x := (v,r)). unfold In. left. reflexivity.
+    apply IHl. 
+    intro. intro.
+    apply H0.
+    unfold In. right. apply H1.
+Qed.
+
+Lemma funspec_interp :
+  forall F f p t,
+    In (f, (p,t)) F -> In (sep_schema f p t) (sep_proc_env F).
+Proof.
+  intros.
+  induction F.
+  + inversion H.
+  + destruct H. destruct a. destruct p1. inversion H. subst.
+    apply in_inv. left. reflexivity.
+    apply IHF in H.
+    unfold sep_proc_env.
+    destruct a.
+    destruct p1.
+    simpl.
+    right.
+    apply H.
+Qed.
+
 Lemma sep_proof_skip :
   forall Φ Γ Γ' (J : (Φ / Γ ⊢ skip_s ::: Γ')), 
-    {{ sep_env Γ }} skip_s {{ sep_env Γ' }}.
+    sep_proc_env Φ |- {{ sep_env Γ }} skip_s {{ sep_env Γ' }}.
 Proof.
   intros. inversion J. constructor.
 Qed.
 
-
 Lemma sep_proof_assign :
   forall Φ Γ Γ' x e (J : (Φ / Γ ⊢ assign_s x e ::: Γ')), 
     wf_env Γ ->
-    {{ sep_env Γ }} assign_s x e {{ sep_env Γ' }}.
+    sep_proc_env Φ |- {{ sep_env Γ }} assign_s x e {{ sep_env Γ' }}.
 Proof.
   intros Φ Γ Γ' x e J wfenv.
   inversion J. subst.
@@ -83,26 +142,297 @@ Proof.
   intros x' x'_in_ctx.
   unfold subst_one. destruct (eq_dec x' x). subst. 
   unfold var_in in *.
-  unfold var_not_in in *. rewrite Forall_forall in H4. destruct (x'_in_ctx). apply H4 in H0. 
-  contradiction H0. reflexivity. reflexivity.
+  unfold var_not_in in *. rewrite Forall_forall in H4. destruct (x'_in_ctx). apply H4 in H. 
+  contradiction H. reflexivity. reflexivity.
   unfold subst_one. destruct (eq_dec ν x). subst. contradiction H1. reflexivity. reflexivity.
   auto.
   apply semax_assign with (e := e) (x := x) (P := (sep_env ((x, {ν : τ | var_e ν .= e}) :: Γ))).
 Qed.
 
+Lemma sep_ty_pure :
+  forall x t,
+    pure (sep_ty x t).
+Proof.
+  intros.
+  unfold pure.
+  intro w.
+  intro.
+  unfold identity.
+  intros w' w''.
+  intro. apply H0.
+Qed.
+
+Lemma sep_ty_pure_subst :
+  forall x t θ,
+    pure (subst θ (sep_ty x t)).
+Proof.
+  intros.
+  unfold pure.
+  intro w.
+  intro.
+  unfold identity.
+  intros w' w''.
+  intro.
+  apply H0.
+Qed.
+
+Lemma sep_env_pure :
+  forall G,
+    pure (sep_env G).
+Proof.
+  intros.
+  unfold pure.
+  intro. intro.
+  unfold identity.
+  intros w1 w2.
+  intros.
+  apply H0.
+Qed.
+
+Lemma sep_args_sub :
+  forall Γ (xs : list var) ts (θ : subst_t var var) S w,
+    length (s_formals S) = length (s_formal_ts S) ->
+    xs = subst θ (s_formals S) ->
+    ts = subst θ (s_formal_ts S) ->
+    tc_list Γ (combine xs ts) ->
+    sep_env Γ w ->
+    sep_env (subst θ (combine (s_formals S) (s_formal_ts S))) w.
+Proof.
+  intros.
+  assert (C: subst θ (combine (s_formals S) (s_formal_ts S)) = 
+                      combine xs ts).
+    rewrite H0. rewrite H1. 
+    rewrite <- subst_combine with (xs := s_formals S) (ys := s_formal_ts S).
+    reflexivity.
+    assumption.
+  rewrite C.
+  apply types_interp with Γ.
+  assumption.
+  assumption.
+Qed.
+
+Lemma sep_env_cons :
+  forall x t Γ w,
+    (sep_ty x t * sep_env Γ)%pred w ->
+    sep_env ((x,t) :: Γ) w.
+Proof.
+  intros.
+  unfold sep_env.
+  split.
+  rewrite sepcon_pure_andp in H.
+  destruct H.
+  apply H.
+  apply sep_ty_pure.
+  apply sep_env_pure.
+  rewrite sepcon_pure_andp in H.
+  destruct H.
+  apply H0.
+  apply sep_ty_pure.
+  apply sep_env_pure.
+Qed.
+  
+Lemma sep_env_cons_sub :
+  forall x b p θ Γ w ,
+    θ ν = ν -> (forall x , θ x = ν -> x = ν) ->
+    ((subst θ (sep_ty x { ν : b | p })) * sep_env Γ)%pred w ->
+    sep_env ((subst θ (x,{ ν : b | p })) :: Γ) w.
+Proof.
+  intros x b p θ Γ w vv_id vv_im.
+  unfold sep_env.
+  intro.
+  rewrite sepcon_pure_andp in H.
+  destruct H.
+  split.
+  unfold subst in H. unfold Subst_pred_var in H.
+  apply subst_ty_distr; assumption.
+  apply H0.
+  apply sep_ty_pure_subst with (t := {ν : b | p}) .
+  apply sep_env_pure.
+Qed.
+
+Lemma sep_proof_proc_ret :
+  forall (θ : subst_t var var) S Γ w, 
+    θ ν = ν -> (forall x, θ x = ν -> x = ν) ->
+    wf_schema S ->
+    wf_type (subst θ (s_ret S) :: Γ) (subst θ (snd (s_ret S)))  ->
+   (((subst θ (sep_ty (fst (s_ret S)) (snd (s_ret S)))) * sep_env Γ)%pred w)  ->
+    (sep_env ((subst θ (s_ret S)) :: Γ) w).
+Proof.
+  intros θ S Γ w vvid vvim wfschema wf H.
+  destruct S as [xs arity [x [ vv b p ]]].
+  inversion wfschema. clear H0 H1. simpl in H2. 
+  inversion H2.
+  inversion H8. subst.
+  unfold s_ret.
+  apply sep_env_cons_sub; assumption.
+Qed.
+
+Lemma sep_proof_proc_sub :
+  forall x v θ,
+    v  = subst θ x ->
+    (forall x', θ x' = v <-> x = x') ->
+    unique_sub θ x.
+Proof.
+  intros x v θ vdef subprop.
+  unfold unique_sub.
+  exists v.
+  split.
+  symmetry. apply vdef.
+  intros.
+  unfold not_free_in.
+  specialize (subprop x0).
+  destruct subprop.
+  intuition.
+  apply H.
+  symmetry.
+  intuition.
+Qed.
+
+Lemma sep_proof_proc_mod :
+  forall f xs x x',
+    modvars (proc_s f xs [x]) x' -> x = x'.
+Proof.
+  intros.
+  inversion H.
+  apply in_inv in H4.
+  intuition.
+Qed.
+
+Ltac wfenv_ty_t :=
+  match goal with 
+    | [ X : ?x = ?a, Y : ?y = ?b, H : wf_type _ _ |- _ ] =>
+      rewrite X in H; rewrite Y in H; assumption
+    | [ H : (?x, ?y) = subst _ (_, _) |- _ ] => 
+      unfold subst, Subst_prod, subst_prod in H; inversion H; wfenv_ty_t
+    | [ H : wf_env (subst ?x (?f ?z) :: ?G) |- wf_type (subst ?x (?f ?z) :: ?G) _ ]  =>
+      inversion H; destruct (f z); simpl in *; wfenv_ty_t
+  end.
+
+Lemma sep_proof_proccall :
+  forall Φ Γ Γ' f xs v (J : (Φ / Γ ⊢ proc_s f xs [v] ::: Γ')),
+    wf_env Γ ->
+    sep_proc_env Φ |- {{ sep_env Γ }} proc_s f xs [v] {{ sep_env Γ' }}.
+Proof.
+  intros. 
+  inversion J. 
+  apply funspec_interp in H3.
+  unfold sep_schema in H3. 
+  apply semax_pre_post with 
+  (P' := (Subst.subst θ (sep_env (combine (s_formals S) (s_formal_ts S)))) * sep_env Γ) 
+  (Q' := (Subst.subst θ (sep_ty (fst (s_ret S)) (snd (s_ret S))))  * sep_env Γ).
+  repeat intro. repeat exists a. 
+  split. unfold join. constructor; reflexivity.
+  split.
+  pose subst_in_env.
+  specialize (i Γ (combine (s_formals S) (s_formal_ts S)) θ a).
+  wfsubst θ.
+  apply i.
+  assumption.
+  assumption.
+  rewrite subst_combine.
+  apply forall_p_combine.
+  inversion H4. repeat rewrite <- subst_length. assumption.
+  rewrite <- H8. assumption.
+  inversion H4. assumption.
+  apply sep_args_sub with (Γ := Γ) (xs := xs) (ts := ts).
+  inversion H4. assumption.
+  assumption.
+  assumption.
+  assumption.
+  assumption.
+  assumption.
+  (**  **)
+  (* inversion H14. *)
+  (* destruct (s_ret S) eqn: sret. *)
+  (* unfold subst, Subst_prod, subst_prod in H18. inversion H18. *)
+  (* rewrite <- H25 in *. *)
+  (* rewrite <- H26 in *. *)
+  (** **)
+  unfold derives.
+  intro w.
+  apply sep_proof_proc_ret.
+  apply wf_subst_split; assumption.
+  apply wf_subst_split; assumption.
+  assumption.
+  wfenv_ty_t.
+  apply semax_frame.
+  subst.
+  destruct S as [ xs ts [x t]].
+  simpl in *.
+  assert (A : subst θ (proc_s f xs [x]) = proc_s f (subst θ xs) [subst θ x]).
+  unfold subst at 1. simpl. reflexivity.
+  rewrite <- A.
+  apply semax_subst.
+  apply (semax_proc f (mkProc (length xs) xs [x] p)).
+  assumption.
+  intros.
+  assert (x = x0) by
+      (apply sep_proof_proc_mod with (f:=f) (xs:= xs); assumption).
+  subst.
+  apply sep_proof_proc_sub with (v := subst θ x0).
+  reflexivity.
+  intros.
+  constructor.
+  intro.
+  specialize (H10 x').
+  symmetry.
+  apply H10.
+  assumption.
+  intro.
+  specialize (H10 x').
+  apply H10.
+  symmetry.
+  assumption.
+  unfold subset.
+  intros.
+  unfold nonfreevars.
+  intros.
+  rewrite subst_dom_env.
+  assumption.
+  assumption.
+  assert (subst θ (fst (s_ret S)) = x) .
+    apply sep_proof_proc_mod with (f:=f) (xs:= (subst θ (s_formals S))). 
+    rewrite <- H9. 
+    rewrite <- H7.
+    assumption.
+  apply subst_one_is_disj.
+  rewrite <- H9 in H20.
+  rewrite H20 in *.
+  destruct S as [fxs fts [xr tr]]. simpl in *.
+  subst.
+  inversion H14. assumption.
+  assumption.
+  destruct S as [fxs fts [xr tr]]. simpl in *.
+  subst.
+  inversion H14.
+  assumption.
+  destruct S as [fx fts [xr tr]]. simpl in *.
+  subst.
+  unfold subst_one.
+  assert (subst θ xr = x) .
+   apply sep_proof_proc_mod with (f:=f) (xs:= (subst θ fx)). assumption.
+  assert (x <> ν).
+  inversion H14. rewrite H0 in H8. assumption.
+  destruct (eq_dec ν x).
+    intuition.
+    reflexivity.
+Qed.
+
 Theorem sep_proof_stmt :
   forall Φ Γ Γ' s (J : (Φ / Γ ⊢ s ::: Γ')),
     wf_env Γ ->
-    {{ sep_env Γ }} s {{ sep_env Γ' }}.
+    sep_proc_env Φ |- {{ sep_env Γ }} s {{ sep_env Γ' }}.
 Proof.
   intros.
   destruct s.
   + apply sep_proof_skip with (Φ := Φ). assumption.
   + apply sep_proof_assign with (Φ := Φ); assumption.
-  + admit.
+  + inversion J. subst. apply sep_proof_proccall with (Φ := Φ); assumption. 
   + induction J.
     * apply semax_skip.
-    * admit.
+    * apply sep_proof_proccall.
+      apply t_proc_s with (p := p) (ts := ts) (θS := θS); assumption.
+      assumption.
     * apply sep_proof_assign with (Φ := Φ). apply t_assign with (φ := φ); assumption. assumption.
     * apply semax_seq with (Q := sep_env Γ'). apply IHJ1. assumption. apply IHJ2. 
       apply wf_env_stmt with (P := Φ) (G := Γ) (s := s0); assumption.
@@ -110,7 +440,7 @@ Qed.
 
 Corollary type_safety :
   forall Φ s Γ,
-    Φ / nil ⊢ s ::: Γ -> {{ TT }} s {{ TT }}.
+    Φ / nil ⊢ s ::: Γ -> sep_proc_env Φ |- {{ TT }} s {{ TT }}.
 Proof.
   intros.
   assert (wf_env nil). constructor.
